Update Equiv_J.v

Equiv_J.v
@@ -2,13 +2,21 @@
 (** * Equiv_J: プログラムの同値性 *)
 
 
-
-Require Export Imp_J.
+Require Import Coq.Bool.Bool.
+Require Import Coq.Arith.Arith.
+Require Import Coq.Arith.EqNat.
+Require Import Coq.omega.Omega.
+Require Import Coq.Lists.List.
+Require Import Coq.Logic.FunctionalExtensionality.
+Import ListNotations.
+Require Import SfLib.
+Require Import Maps.
+Require Import Imp.
 
 (*  *** Some general advice for working on exercises:
 
     - Most of the Coq proofs we ask you to do are similar to proofs
-      that we've provided.  Before starting to work on the homework
+      that we've provided.  Before starting to work on exercises
       problems, take the time to work through our proofs (both
       informally, on paper, and in Coq) and make sure you understand
       them in detail.  This will save you a lot of time.
@@ -50,23 +58,23 @@ Require Export Imp_J.
 (* * Behavioral Equivalence *)
 (** * 振る舞い同値性 *)
 
-(* In the last chapter, we investigated the correctness of a very
+(* In an earlier chapter, we investigated the correctness of a very
     simple program transformation: the [optimize_0plus] function.  The
     programming language we were considering was the first version of
     the language of arithmetic expressions -- with no variables -- so
-    in that setting it was very easy to define what it _means_ for a
+    in that setting it was very easy to define what it means for a
     program transformation to be correct: it should always yield a
-    program that evaluates to the same number as the original.  
+    program that evaluates to the same number as the original.
 
     To go further and talk about the correctness of program
     transformations in the full Imp language, we need to consider the
     role of variables and state. *)
 
-(** 前の章で、簡単なプログラム変換の正しさを調べました。
+(** 以前の章で、簡単なプログラム変換の正しさを調べました。
     [optimize_0plus]関数です。
     対象としたプログラミング言語は、算術式の言語の最初のバージョンでした。
-    それには変数もなく、そのためプログラム変換が正しいとはどういうことを意味する(_means_)
-    かを定義することはとても簡単でした。
+    それには変数もなく、そのためプログラム変換が正しいとはどういうことかという意味
+    を定義することはとても簡単でした。
     つまり、変換の結果得られるプログラムが常に、
     それを評価すると元のプログラムと同じ数値になるということでした。
 
@@ -83,30 +91,30 @@ Require Export Imp_J.
     evaluate to the same result _in every state_. *)
 (** 変数を伴う[aexp]と[bexp]については、どう定義すれば良いかは明らかです。
     2つの[aexp]または[bexp]が振る舞い同値である(_behaviorally equivalent_)とは、
-    「すべての状態で」2つの評価結果が同じになることです。*)    
- 
+    「すべての状態で」2つの評価結果が同じになることです。*)   
+
 Definition aequiv (a1 a2 : aexp) : Prop :=
-  forall (st:state), 
+  forall (st:state),
     aeval st a1 = aeval st a2.
 
 Definition bequiv (b1 b2 : bexp) : Prop :=
-  forall (st:state), 
+  forall (st:state),
     beval st b1 = beval st b2.
 
-(* For commands, the situation is a little more subtle.  We can't
+(*  For commands, the situation is a little more subtle.  We can't
     simply say "two commands are behaviorally equivalent if they
     evaluate to the same ending state whenever they are started in the
-    same initial state," because some commands (in some starting
-    states) don't terminate in any final state at all!  What we need
-    instead is this: two commands are behaviorally equivalent if, for
-    any given starting state, they either both diverge or both
+    same initial state," because some commands, when run in some
+    starting states, don't terminate in any final state at all!  What
+    we need instead is this: two commands are behaviorally equivalent
+    if, for any given starting state, they either both diverge or both
     terminate in the same final state.  A compact way to express this
     is "if the first one terminates in a particular state then so does
     the second, and vice versa." *)
 (** コマンドについては、状況はもうちょっと微妙です。
     簡単に「2つのコマンドが振る舞い同値であるとは、
     両者を同じ状態から開始すれば同じ状態で終わることである」と言うわけには行きません。
-    コマンドによっては(特定の状態から開始したときには)
+    コマンドによっては,特定の状態から開始したときには、
     停止しないためどのような状態にもならないことがあるからです!
     すると次のように言う必要があります。
     2つのコマンドが振る舞い同値であるとは、任意の与えられた状態から両者をスタートすると、
@@ -115,25 +123,22 @@ Definition bequiv (b1 b2 : bexp) : Prop :=
     逆もまた成り立つ」となります。*)
 
 Definition cequiv (c1 c2 : com) : Prop :=
-  forall (st st' : state), 
-    (c1 / st || st') <-> (c2 / st || st').
+  forall (st st' : state),
+    (c1 / st \\ st') <-> (c2 / st \\ st').
 
-
-
-(*  **** Exercise: 2 stars (equiv_classes)  *)
 (** **** 練習問題: ★★, (equiv_classes) *)
 
 (*  Given the following programs, group together those that are
-    equivalent in [Imp]. Your answer should be given as a list of
-    lists, where each sub-list represents a group of equivalent
-    programs. For example, if you think programs (a) through (h) are
-    all equivalent to each other, but not to (i), your answer should
-    look like this:
+    equivalent in Imp. Your answer should be given as a list of lists,
+    where each sub-list represents a group of equivalent programs. For
+    example, if you think programs (a) through (h) are all equivalent
+    to each other, but not to (i), your answer should look like this:
 
-    [ [prog_a;prog_b;prog_c;prog_d;prog_e;prog_f;prog_g;prog_h] ;
-      [prog_i] ]
+       [ [prog_a;prog_b;prog_c;prog_d;prog_e;prog_f;prog_g;prog_h] ;
+         [prog_i] ]
 
-    Write down your answer below in the definition of [equiv_classes]. *)
+    Write down your answer below in the definition of
+    [equiv_classes]. *)
 (** 次のプログラムが与えられたとき、[Imp]において等しいものグループを作りなさい。
     あなたの答をリストのリストとして表現し、それぞれのサブリストが等価なプログラムのグループを表すようにしなさい。例えば、(a)から(h)までが全て同じプログラムであり、(i)だけが違うと思うならば、答は次のようになります：
 
@@ -191,7 +196,6 @@ Definition prog_i : com :=
 
 Definition equiv_classes : list (list com) :=
 (* FILL IN HERE *) admit.
-(* GRADE_TEST 2: check_equiv_classes equiv_classes *)
 (** [] *)
 
 (* ####################################################### *)
@@ -205,12 +209,12 @@ Definition equiv_classes : list (list com) :=
 Theorem aequiv_example:
   aequiv (AMinus (AId X) (AId X)) (ANum 0).
 Proof.
-  intros st. simpl. apply minus_diag.
+  intros st. simpl. omega.
 Qed.
 
 Theorem bequiv_example:
-  bequiv (BEq (AMinus (AId X) (AId X)) (ANum 0)) BTrue. 
-Proof. 
+  bequiv (BEq (AMinus (AId X) (AId X)) (ANum 0)) BTrue.
+Proof.
   intros st. unfold beval.
   rewrite aequiv_example. reflexivity.
 Qed.
@@ -221,54 +225,51 @@ Qed.
     [SKIP]にからんだ自明な変換から見てみましょう: *)
 
 Theorem skip_left: forall c,
-  cequiv 
-     (SKIP;; c) 
+  cequiv
+     (SKIP;; c)
      c.
-Proof. 
+Proof.
   (* WORKED IN CLASS *)
   intros c st st'.
   split; intros H.
-  Case "->". 
-    inversion H. subst. 
-    inversion H2. subst. 
+  - (* -> *)
+    inversion H. subst.
+    inversion H2. subst.
     assumption.
-  Case "<-". 
+  - (* <- *)
     apply E_Seq with st.
-    apply E_Skip. 
-    assumption.  
+    apply E_Skip.
+    assumption.
 Qed.
 
-(* **** Exercise: 2 stars (skip_right) *)
 (** **** 練習問題: ★★ (skip_right) *)
-(*  Prove that adding a SKIP after a command results in an equivalent
-    program *)
+(*  Prove that adding a [SKIP] after a command results in an
+    equivalent program *)
 (** SKIPをコマンドの結果の後ろに追加することはもとのプログラムと等しいことを証明しなさい *)
 
-
 Theorem skip_right: forall c,
-  cequiv 
-    (c;; SKIP) 
+  cequiv
+    (c ;; SKIP)
     c.
-Proof. 
+Proof.
   (* FILL IN HERE *) Admitted.
 (** [] *)
 
-(** Similarly, here is a simple transformations that simplifies [IFB]
+(** Similarly, here is a simple transformations that optimizes [IFB]
     commands: *)
-(** 同様に[IFB]コマンドを簡単化する単純な変換です: *)
+(** 同様に[IFB]コマンドを最適化する単純な変換です: *)
 
 Theorem IFB_true_simple: forall c1 c2,
-  cequiv 
-    (IFB BTrue THEN c1 ELSE c2 FI) 
+  cequiv
+    (IFB BTrue THEN c1 ELSE c2 FI)
     c1.
-Proof. 
-  intros c1 c2. 
+Proof.
+  intros c1 c2.
   split; intros H.
-  Case "->".
+  - (* -> *)
     inversion H; subst. assumption. inversion H5.
-  Case "<-".
+  - (* <- *)
     apply E_IfTrue. reflexivity. assumption.  Qed.
-
 
 (*  Of course, few programmers would be tempted to write a conditional
     whose guard is literally [BTrue].  A more interesting case is when
@@ -284,25 +285,25 @@ Proof.
 *)
 (** *** *)
 (**
-   _Proof_: 
+   _Proof_:
 
      - ([->]) We must show, for all [st] and [st'], that if [IFB b
-       THEN c1 ELSE c2 FI / st || st'] then [c1 / st || st'].
+       THEN c1 ELSE c2 FI / st \\ st'] then [c1 / st \\ st'].
 
        Proceed by cases on the rules that could possibly have been
-       used to show [IFB b THEN c1 ELSE c2 FI / st || st'], namely
+       used to show [IFB b THEN c1 ELSE c2 FI / st \\ st'], namely
        [E_IfTrue] and [E_IfFalse].
 
        - Suppose the final rule rule in the derivation of [IFB b THEN
-         c1 ELSE c2 FI / st || st'] was [E_IfTrue].  We then have, by
-         the premises of [E_IfTrue], that [c1 / st || st'].  This is
+         c1 ELSE c2 FI / st \\ st'] was [E_IfTrue].  We then have, by
+         the premises of [E_IfTrue], that [c1 / st \\ st'].  This is
          exactly what we set out to prove.
 
        - On the other hand, suppose the final rule in the derivation
-         of [IFB b THEN c1 ELSE c2 FI / st || st'] was [E_IfFalse].
-         We then know that [beval st b = false] and [c2 / st || st'].
+         of [IFB b THEN c1 ELSE c2 FI / st \\ st'] was [E_IfFalse].
+         We then know that [beval st b = false] and [c2 / st \\ st'].
 
-         Recall that [b] is equivalent to [BTrue], i.e. forall [st],
+         Recall that [b] is equivalent to [BTrue], i.e., forall [st],
          [beval st b = beval st BTrue].  In particular, this means
          that [beval st b = true], since [beval st BTrue = true].  But
          this is a contradiction, since [E_IfFalse] requires that
@@ -310,31 +311,31 @@ Proof.
          been [E_IfFalse].
 
      - ([<-]) We must show, for all [st] and [st'], that if [c1 / st
-       || st'] then [IFB b THEN c1 ELSE c2 FI / st || st'].
+       \\ st'] then [IFB b THEN c1 ELSE c2 FI / st \\ st'].
 
        Since [b] is equivalent to [BTrue], we know that [beval st b] =
        [beval st BTrue] = [true].  Together with the assumption that
-       [c1 / st || st'], we can apply [E_IfTrue] to derive [IFB b THEN
-       c1 ELSE c2 FI / st || st'].  []
+       [c1 / st \\ st'], we can apply [E_IfTrue] to derive [IFB b THEN
+       c1 ELSE c2 FI / st \\ st'].  []
 
    Here is the formal version of this proof: *)
-(** 
+(**
    「証明」:
 
-     - ([->]) すべての[st]と[st']に対して、もし[IFB b THEN c1 ELSE c2 FI / st || st']
-       ならば[c1 / st || st']となることを示す。
+     - ([->]) すべての[st]と[st']に対して、もし[IFB b THEN c1 ELSE c2 FI / st \\ st']
+       ならば[c1 / st \\ st']となることを示す。
 
-       [IFB b THEN c1 ELSE c2 FI / st || st']を示すのに使うことができた可能性のある規則、
+       [IFB b THEN c1 ELSE c2 FI / st \\ st']を示すのに使うことができた可能性のある規則、
        つまり[E_IfTrue]と[E_IfFalse]とで、場合分けをする。
 
-       - [IFB b THEN c1 ELSE c2 FI / st || st']
+       - [IFB b THEN c1 ELSE c2 FI / st \\ st']
          の導出の最後の規則が[E_IfTrue]であると仮定する。
-         このとき、[E_IfTrue]の仮定より[c1 / st || st']となる。
+         このとき、[E_IfTrue]の仮定より[c1 / st \\ st']となる。
          これはまさに証明したいことである。
 
-       - 一方、[IFB b THEN c1 ELSE c2 FI / st || st']
+       - 一方、[IFB b THEN c1 ELSE c2 FI / st \\ st']
          の導出の最後の規則が[E_IfFalse]と仮定する。
-         すると、[beval st b = false]かつ[c2 / st || st']となる。
+         すると、[beval st b = false]かつ[c2 / st \\ st']となる。
 
          [b]が[BTrue]と同値であったことから、
          すべての[st]について、[beval st b = beval st BTrue]が成立する。
@@ -344,34 +345,34 @@ Proof.
          [E_IfFalse]から[beval st b = false]でなければならないからである。
          従って、最後の規則は[E_IfFalse]ではあり得ない。
 
-     - ([<-]) すべての[st]と[st']について、もし[c1 / st|| st']ならば
-       [IFB b THEN c1 ELSE c2 FI / st || st']となることを示す。
+     - ([<-]) すべての[st]と[st']について、もし[c1 / st\\ st']ならば
+       [IFB b THEN c1 ELSE c2 FI / st \\ st']となることを示す。
 
        [b]が[BTrue]と同値であることから、
        [beval st b] = [beval st BTrue] = [true]となる。
-       仮定[c1 / st || st']より[E_IfTrue]が適用でき、
-       [IFB b THEN c1 ELSE c2 FI / st || st']となる。  []
-       
+       仮定[c1 / st \\ st']より[E_IfTrue]が適用でき、
+       [IFB b THEN c1 ELSE c2 FI / st \\ st']となる。  []
+      
 
    以下がこの証明の形式化版です: *)
 
 Theorem IFB_true: forall b c1 c2,
      bequiv b BTrue  ->
-     cequiv 
-       (IFB b THEN c1 ELSE c2 FI) 
+     cequiv
+       (IFB b THEN c1 ELSE c2 FI)
        c1.
 Proof.
   intros b c1 c2 Hb.
   split; intros H.
-  Case "->".
+  - (* -> *)
     inversion H; subst.
-    SCase "b evaluates to true".
+    + (* b evaluates to true *)
       assumption.
-    SCase "b evaluates to false (contradiction)".
+    + (* b evaluates to false (contradiction) *)
       unfold bequiv in Hb. simpl in Hb.
       rewrite Hb in H5.
       inversion H5.
-  Case "<-".
+  - (* <- *)
     apply E_IfTrue; try assumption.
     unfold bequiv in Hb. simpl in Hb.
     rewrite Hb. reflexivity.  Qed.
@@ -380,8 +381,8 @@ Proof.
 (** **** 練習問題: ★★ (IFB_false) *)
 Theorem IFB_false: forall b c1 c2,
   bequiv b BFalse  ->
-  cequiv 
-    (IFB b THEN c1 ELSE c2 FI) 
+  cequiv
+    (IFB b THEN c1 ELSE c2 FI)
     c2.
 Proof.
   (* FILL IN HERE *) Admitted.
@@ -418,15 +419,15 @@ Theorem WHILE_false : forall b c,
      cequiv
        (WHILE b DO c END)
        SKIP.
-Proof. 
+Proof.
   intros b c Hb. split; intros H.
-  Case "->".
+  - (* -> *)
     inversion H; subst.
-    SCase "E_WhileEnd".
+    + (* E_WhileEnd *)
       apply E_Skip.
-    SCase "E_WhileLoop".
+    + (* E_WhileLoop *)
       rewrite Hb in H2. inversion H2.
-  Case "<-".
+  - (* <- *)
     inversion H; subst.
     apply E_WhileEnd.
     rewrite Hb.
@@ -450,67 +451,67 @@ Proof.
     terminate:
 
     _Lemma_: If [b] is equivalent to [BTrue], then it cannot be the
-    case that [(WHILE b DO c END) / st || st'].
+    case that [(WHILE b DO c END) / st \\ st'].
 
-    _Proof_: Suppose that [(WHILE b DO c END) / st || st'].  We show,
-    by induction on a derivation of [(WHILE b DO c END) / st || st'],
-    that this assumption leads to a contradiction.  
+    _Proof_: Suppose that [(WHILE b DO c END) / st \\ st'].  We show,
+    by induction on a derivation of [(WHILE b DO c END) / st \\ st'],
+    that this assumption leads to a contradiction. 
 
-      - Suppose [(WHILE b DO c END) / st || st'] is proved using rule
+      - Suppose [(WHILE b DO c END) / st \\ st'] is proved using rule
         [E_WhileEnd].  Then by assumption [beval st b = false].  But
         this contradicts the assumption that [b] is equivalent to
         [BTrue].
 
-      - Suppose [(WHILE b DO c END) / st || st'] is proved using rule
+      - Suppose [(WHILE b DO c END) / st \\ st'] is proved using rule
         [E_WhileLoop].  Then we are given the induction hypothesis
-        that [(WHILE b DO c END) / st || st'] is contradictory, which
+        that [(WHILE b DO c END) / st \\ st'] is contradictory, which
         is exactly what we are trying to prove!
 
       - Since these are the only rules that could have been used to
-        prove [(WHILE b DO c END) / st || st'], the other cases of
+        prove [(WHILE b DO c END) / st \\ st'], the other cases of
         the induction are immediately contradictory. [] *)
 (** 2つ目の事実を証明するためには、
     ガードが[BTrue]と同値であるwhileループが停止しないことを言う補題が1つ必要です:
 
     「補題」:[b]が[BTrue]と同値のとき、
-    [(WHILE b DO c END) / st || st']となることはない。
+    [(WHILE b DO c END) / st \\ st']となることはない。
 
-    「証明」:[(WHILE b DO c END) / st || st']と仮定する。
-    [(WHILE b DO c END) / st || st']の導出についての帰納法によって、
+    「証明」:[(WHILE b DO c END) / st \\ st']と仮定する。
+    [(WHILE b DO c END) / st \\ st']の導出についての帰納法によって、
     この仮定から矛盾が導かれることを示す。
 
-      - [(WHILE b DO c END) / st || st']が規則[E_WhileEnd]
+      - [(WHILE b DO c END) / st \\ st']が規則[E_WhileEnd]
         から証明されると仮定する。すると仮定から[beval st b = false]となる。
         しかしこれは、[b]が[BTrue]と同値という仮定と矛盾する。
 
-      - [(WHILE b DO c END) / st || st']が規則[E_WhileLoop]
+      - [(WHILE b DO c END) / st \\ st']が規則[E_WhileLoop]
         を使って証明されると仮定する。
         すると帰納法の仮定として
-        [(WHILE b DO c END) / st || st']が矛盾するということが得られる。
+        [(WHILE b DO c END) / st \\ st']が矛盾するということが得られる。
         これはまさに証明しようとしていることである。
 
-      - 上記が[(WHILE b DO c END) / st || st']
+      - 上記が[(WHILE b DO c END) / st \\ st']
         の証明に使うことができる可能性がある規則のすべてであり、
         帰納法の他の場合は、すぐに矛盾になる。[] *)
 
 Lemma WHILE_true_nonterm : forall b c st st',
      bequiv b BTrue ->
-     ~( (WHILE b DO c END) / st || st' ).
-Proof. 
+     ~( (WHILE b DO c END) / st \\ st' ).
+Proof.
   (* WORKED IN CLASS *)
   intros b c st st' Hb.
   intros H.
   remember (WHILE b DO c END) as cw eqn:Heqcw.
   ceval_cases (induction H) Case;
-    (* Most rules don't apply, and we can rule them out 
+    (* Most rules don't apply, and we can rule them out
        by inversion *)
     inversion Heqcw; subst; clear Heqcw.
   (* The two interesting cases are the ones for WHILE loops: *)
-  Case "E_WhileEnd". (* contradictory -- b is always true! *)
+  - (* E_WhileEnd *) (* contradictory -- b is always true! *)
     unfold bequiv in Hb.
     (* [rewrite] is able to instantiate the quantifier in [st] *)
     rewrite Hb in H. inversion H.
-  Case "E_WhileLoop". (* immediate from the IH *)
+  - (* E_WhileLoop *) (* immediate from the IH *)
     apply IHceval2. reflexivity.  Qed.
 
 (* **** Exercise: 2 stars, optional (WHILE_true_nonterm_informal) *)
@@ -532,10 +533,10 @@ Proof.
 
 Theorem WHILE_true: forall b c,
      bequiv b BTrue  ->
-     cequiv 
+     cequiv
        (WHILE b DO c END)
        (WHILE BTrue DO SKIP END).
-Proof. 
+Proof.
   (* FILL IN HERE *) Admitted.
 (** [] *)
 
@@ -547,20 +548,20 @@ Proof.
   (* WORKED IN CLASS *)
   intros b c st st'.
   split; intros Hce.
-  Case "->".
-    inversion Hce; subst.  
-    SCase "loop doesn't run".
+  - (* -> *)
+    inversion Hce; subst. 
+    + (* loop doesn't run *)
       apply E_IfFalse. assumption. apply E_Skip.
-    SCase "loop runs".
+    + (* loop runs *)
       apply E_IfTrue. assumption.
       apply E_Seq with (st' := st'0). assumption. assumption.
-  Case "<-".
+  - (* <- *)
     inversion Hce; subst.
-    SCase "loop runs".
+    + (* loop runs *)
       inversion H5; subst.
-      apply E_WhileLoop with (st' := st'0). 
+      apply E_WhileLoop with (st' := st'0).
       assumption. assumption. assumption.
-    SCase "loop doesn't run".
+    + (* loop doesn't run *)
       inversion H5; subst. apply E_WhileEnd. assumption.  Qed.
 
 (* **** Exercise: 2 stars, optional (seq_assoc) *)
@@ -584,12 +585,12 @@ Proof.
 
 Theorem identity_assignment_first_try : forall (X:id),
   cequiv (X ::= AId X) SKIP.
-Proof. 
+Proof.
    intros. split; intro H.
-     Case "->". 
+     - (* -> *)
        inversion H; subst.  simpl.
-       replace (update st X (st X)) with st.  
-       constructor. 
+       replace (update st X (st X)) with st. 
+       constructor.
        (* 詰った... *) Abort.
 
 (*  Here we're stuck. The goal looks reasonable, but in fact it is not
@@ -627,7 +628,7 @@ Proof.
     or
     cequiv (X ::= 1;; Y ::= 2)
            (y ::= 2;; X ::= 1)
-  
+ 
     we'll get stuck in the same way: we'll have two functions that
     behave the same way on all inputs, but cannot be proven to be [eq]
     to each other.
@@ -668,7 +669,7 @@ Proof.
                         -------------------
                                f = g
     この原理は Coq のビルトインの論理からは導出できませんが、
-    追加公理(_axiom_)として導入することは安全です。*)    
+    追加公理(_axiom_)として導入することは安全です。*)   
 
 Axiom functional_extensionality : forall {X Y: Type} {f g : X -> Y},
     (forall (x: X), f x = g x) ->  f = g.
@@ -687,27 +688,27 @@ Theorem identity_assignment : forall (X:id),
   cequiv
     (X ::= AId X)
     SKIP.
-Proof. 
+Proof.
    intros. split; intro H.
-     Case "->". 
+     - (* -> *)
        inversion H; subst. simpl.
-       replace (update st X (st X)) with st.  
-       constructor. 
-       apply functional_extensionality. intro. 
-       rewrite update_same; reflexivity.  
-     Case "<-".
-       inversion H; subst. 
+       replace (update st X (st X)) with st. 
+       constructor.
+       apply functional_extensionality. intro.
+       rewrite update_same; reflexivity. 
+     - (* <- *)
+       inversion H; subst.
        assert (st' = (update st' X (st' X))).
-          apply functional_extensionality. intro. 
+          apply functional_extensionality. intro.
           rewrite update_same; reflexivity.
-       rewrite H0 at 2. 
+       rewrite H0 at 2.
        constructor. reflexivity.
 Qed.
 
 (*  **** Exercise: 2 stars (assign_aequiv)  *)
 (** **** 練習問題: ★★ (assign_aequiv) *)
 Theorem assign_aequiv : forall X e,
-  aequiv (AId X) e -> 
+  aequiv (AId X) e ->
   cequiv SKIP (X ::= e).
 Proof.
   (* FILL IN HERE *) Admitted.
@@ -735,13 +736,13 @@ Lemma refl_aequiv : forall (a : aexp), aequiv a a.
 Proof.
   intros a st. reflexivity.  Qed.
 
-Lemma sym_aequiv : forall (a1 a2 : aexp), 
+Lemma sym_aequiv : forall (a1 a2 : aexp),
   aequiv a1 a2 -> aequiv a2 a1.
 Proof.
   intros a1 a2 H. intros st. symmetry. apply H.  Qed.
 
-Lemma trans_aequiv : forall (a1 a2 a3 : aexp), 
-  aequiv a1 a2 -> aequiv a2 a3 -> aequiv a1 a3. 
+Lemma trans_aequiv : forall (a1 a2 a3 : aexp),
+  aequiv a1 a2 -> aequiv a2 a3 -> aequiv a1 a3.
 Proof.
   unfold aequiv. intros a1 a2 a3 H12 H23 st.
   rewrite (H12 st). rewrite (H23 st). reflexivity.  Qed.
@@ -750,13 +751,13 @@ Lemma refl_bequiv : forall (b : bexp), bequiv b b.
 Proof.
   unfold bequiv. intros b st. reflexivity.  Qed.
 
-Lemma sym_bequiv : forall (b1 b2 : bexp), 
+Lemma sym_bequiv : forall (b1 b2 : bexp),
   bequiv b1 b2 -> bequiv b2 b1.
 Proof.
   unfold bequiv. intros b1 b2 H. intros st. symmetry. apply H.  Qed.
 
-Lemma trans_bequiv : forall (b1 b2 b3 : bexp), 
-  bequiv b1 b2 -> bequiv b2 b3 -> bequiv b1 b3. 
+Lemma trans_bequiv : forall (b1 b2 b3 : bexp),
+  bequiv b1 b2 -> bequiv b2 b3 -> bequiv b1 b3.
 Proof.
   unfold bequiv. intros b1 b2 b3 H12 H23 st.
   rewrite (H12 st). rewrite (H23 st). reflexivity.  Qed.
@@ -765,29 +766,29 @@ Lemma refl_cequiv : forall (c : com), cequiv c c.
 Proof.
   unfold cequiv. intros c st st'. apply iff_refl.  Qed.
 
-Lemma sym_cequiv : forall (c1 c2 : com), 
+Lemma sym_cequiv : forall (c1 c2 : com),
   cequiv c1 c2 -> cequiv c2 c1.
 Proof.
   unfold cequiv. intros c1 c2 H st st'.
-  assert (c1 / st || st' <-> c2 / st || st') as H'. 
-    SCase "Proof of assertion". apply H.
+  assert (c1 / st \\ st' <-> c2 / st \\ st') as H'.
+    + (* Proof of assertion *) apply H.
   apply iff_sym. assumption.
 Qed.
 
-Lemma iff_trans : forall (P1 P2 P3 : Prop), 
+Lemma iff_trans : forall (P1 P2 P3 : Prop),
   (P1 <-> P2) -> (P2 <-> P3) -> (P1 <-> P3).
 Proof.
   intros P1 P2 P3 H12 H23.
   inversion H12. inversion H23.
-  split; intros A. 
+  split; intros A.
     apply H1. apply H. apply A.
     apply H0. apply H2. apply A.  Qed.
 
-Lemma trans_cequiv : forall (c1 c2 c3 : com), 
-  cequiv c1 c2 -> cequiv c2 c3 -> cequiv c1 c3. 
+Lemma trans_cequiv : forall (c1 c2 c3 : com),
+  cequiv c1 c2 -> cequiv c2 c3 -> cequiv c1 c3.
 Proof.
   unfold cequiv. intros c1 c2 c3 H12 H23 st st'.
-  apply iff_trans with (c2 / st || st'). apply H12. apply H23.  Qed.
+  apply iff_trans with (c2 / st \\ st'). apply H12. apply H23.  Qed.
 
 (* ######################################################## *)
 (* ** Behavioral Equivalence is a Congruence *)
@@ -799,12 +800,12 @@ Proof.
               aequiv a1 a1'
       -----------------------------
       cequiv (i ::= a1) (i ::= a1')
- 
-              cequiv c1 c1'    
+
+              cequiv c1 c1'   
               cequiv c2 c2'
          ------------------------
          cequiv (c1;;c2) (c1';;c2')
-    ...and so on.  
+    ...and so on. 
 
     (Note that we are using the inference rule notation here not as
     part of a definition, but simply to write down some valid
@@ -850,10 +851,10 @@ Theorem CAss_congruence : forall i a1 a1',
 Proof.
   intros i a1 a2 Heqv st st'.
   split; intros Hceval.
-  Case "->".
-    inversion Hceval. subst. apply E_Ass. 
+  - (* -> *)
+    inversion Hceval. subst. apply E_Ass.
     rewrite Heqv. reflexivity.
-  Case "<-".
+  - (* <- *)
     inversion Hceval. subst. apply E_Ass.
     rewrite Heqv. reflexivity.  Qed.
 
@@ -866,12 +867,12 @@ Proof.
 
     _Proof_: Suppose [b1] is equivalent to [b1'] and [c1] is
     equivalent to [c1'].  We must show, for every [st] and [st'], that
-    [WHILE b1 DO c1 END / st || st'] iff [WHILE b1' DO c1' END / st
-    || st'].  We consider the two directions separately.
+    [WHILE b1 DO c1 END / st \\ st'] iff [WHILE b1' DO c1' END / st
+    \\ st'].  We consider the two directions separately.
 
-      - ([->]) We show that [WHILE b1 DO c1 END / st || st'] implies
-        [WHILE b1' DO c1' END / st || st'], by induction on a
-        derivation of [WHILE b1 DO c1 END / st || st'].  The only
+      - ([->]) We show that [WHILE b1 DO c1 END / st \\ st'] implies
+        [WHILE b1' DO c1' END / st \\ st'], by induction on a
+        derivation of [WHILE b1 DO c1 END / st \\ st'].  The only
         nontrivial cases are when the final rule in the derivation is
         [E_WhileEnd] or [E_WhileLoop].
 
@@ -879,18 +880,18 @@ Proof.
             [beval st b1 = false] and [st = st'].  But then, since
             [b1] and [b1'] are equivalent, we have [beval st b1' =
             false], and [E-WhileEnd] applies, giving us [WHILE b1' DO
-            c1' END / st || st'], as required.
+            c1' END / st \\ st'], as required.
 
           - [E_WhileLoop]: The form of the rule now gives us [beval st
-            b1 = true], with [c1 / st || st'0] and [WHILE b1 DO c1
-            END / st'0 || st'] for some state [st'0], with the
-            induction hypothesis [WHILE b1' DO c1' END / st'0 ||
-            st'].  
+            b1 = true], with [c1 / st \\ st'0] and [WHILE b1 DO c1
+            END / st'0 \\ st'] for some state [st'0], with the
+            induction hypothesis [WHILE b1' DO c1' END / st'0 \\
+            st']. 
 
             Since [c1] and [c1'] are equivalent, we know that [c1' /
-            st || st'0].  And since [b1] and [b1'] are equivalent, we
+            st \\ st'0].  And since [b1] and [b1'] are equivalent, we
             have [beval st b1' = true].  Now [E-WhileLoop] applies,
-            giving us [WHILE b1' DO c1' END / st || st'], as
+            giving us [WHILE b1' DO c1' END / st \\ st'], as
             required.
 
       - ([<-]) Similar. [] *)
@@ -902,13 +903,13 @@ Proof.
 
     「証明」:[b1]が[b1']と同値、[c1]が[c1']と同値であるとする。
     すべての[st]と[st']について、証明すべきことは、
-    [WHILE b1 DO c1 END / st || st']の必要十分条件は
-    [WHILE b1' DO c1' END / st || st']であることである。
+    [WHILE b1 DO c1 END / st \\ st']の必要十分条件は
+    [WHILE b1' DO c1' END / st \\ st']であることである。
     必要条件と十分条件の両方向を別々に証明する。
 
-      - ([->]) [WHILE b1 DO c1 END / st || st']ならば
-        [WHILE b1' DO c1' END / st || st']であることを、
-        [WHILE b1 DO c1 END / st || st']の導出についての帰納法で示す。
+      - ([->]) [WHILE b1 DO c1 END / st \\ st']ならば
+        [WHILE b1' DO c1' END / st \\ st']であることを、
+        [WHILE b1 DO c1 END / st \\ st']の導出についての帰納法で示す。
         自明でないのは、導出の最後の規則が[E_WhileEnd]または[E_WhileLoop]のときだけである。
 
           - [E_WhileEnd]: この場合、
@@ -916,17 +917,17 @@ Proof.
             しかし[b1]と[b1']が同値であることから
             [beval st b1' = false]になる。
             さらに[E-WhileEnd]を適用すると
-            証明すべき[WHILE b1' DO c1' END / st || st']が得られる。
+            証明すべき[WHILE b1' DO c1' END / st \\ st']が得られる。
 
           - [E_WhileLoop]: 規則の形から
             [beval st b1 = true]および、ある状態[st'0]について
-            帰納法の仮定[WHILE b1' DO c1' END / st'0 || st']のもとで、
-            [c1 / st || st'0]かつ[WHILE b1 DO c1 END / st'0 || st']となる。
+            帰納法の仮定[WHILE b1' DO c1' END / st'0 \\ st']のもとで、
+            [c1 / st \\ st'0]かつ[WHILE b1 DO c1 END / st'0 \\ st']となる。
 
-            [c1]と[c1']が同値であることから、[c1' / st || st'0]となる。
+            [c1]と[c1']が同値であることから、[c1' / st \\ st'0]となる。
             さらに[b1]と[b1']が同値であることから、[beval st b1' = true]となる。
             [E-WhileLoop]を適用すると、
-            証明すべき[WHILE b1' DO c1' END / st || st']が得られる。
+            証明すべき[WHILE b1' DO c1' END / st \\ st']が得られる。
 
       - ([<-]) 同様である。
 
@@ -940,50 +941,49 @@ Proof.
   unfold bequiv,cequiv.
   intros b1 b1' c1 c1' Hb1e Hc1e st st'.
   split; intros Hce.
-  Case "->".
-    remember (WHILE b1 DO c1 END) as cwhile eqn:Heqcwhile.
+  - (* -> *)
+    remember (WHILE b1 DO c1 END) as cwhile
+      eqn:Heqcwhile.
     induction Hce; inversion Heqcwhile; subst.
-    SCase "E_WhileEnd".
+    + (* E_WhileEnd *)
       apply E_WhileEnd. rewrite <- Hb1e. apply H.
-    SCase "E_WhileLoop".
+    + (* E_WhileLoop *)
       apply E_WhileLoop with (st' := st').
-      SSCase "show loop runs". rewrite <- Hb1e. apply H.
-      SSCase "body execution". 
-        apply (Hc1e st st').  apply Hce1. 
-      SSCase "subsequent loop execution".
+      * (* show loop runs *) rewrite <- Hb1e. apply H.
+      * (* body execution *)
+        apply (Hc1e st st').  apply Hce1.
+      * (* subsequent loop execution *)
         apply IHHce2. reflexivity.
-  Case "<-".
-    remember (WHILE b1' DO c1' END) as c'while eqn:Heqc'while.
+  - (* <- *)
+    remember (WHILE b1' DO c1' END) as c'while
+      eqn:Heqc'while.
     induction Hce; inversion Heqc'while; subst.
-    SCase "E_WhileEnd".
+    + (* E_WhileEnd *)
       apply E_WhileEnd. rewrite -> Hb1e. apply H.
-    SCase "E_WhileLoop".
+    + (* E_WhileLoop *)
       apply E_WhileLoop with (st' := st').
-      SSCase "show loop runs". rewrite -> Hb1e. apply H.
-      SSCase "body execution". 
-        apply (Hc1e st st').  apply Hce1. 
-      SSCase "subsequent loop execution".
+      * (* show loop runs *) rewrite -> Hb1e. apply H.
+      * (* body execution *)
+        apply (Hc1e st st').  apply Hce1.
+      * (* subsequent loop execution *)
         apply IHHce2. reflexivity.  Qed.
 
-(* **** Exercise: 3 stars, optional (CSeq_congruence) *)
 (** **** 練習問題: ★★★, optional (CSeq_congruence) *)
 Theorem CSeq_congruence : forall c1 c1' c2 c2',
   cequiv c1 c1' -> cequiv c2 c2' ->
   cequiv (c1;;c2) (c1';;c2').
-Proof. 
-  (* FILL IN HERE *) Admitted.
-(** [] *)
-
-(* **** Exercise: 3 stars (CIf_congruence) *)
-(** **** 練習問題: ★★★ (CIf_congruence) *)
-Theorem CIf_congruence : forall b b' c1 c1' c2 c2',
-  bequiv b b' -> cequiv c1 c1' -> cequiv c2 c2' ->
-  cequiv (IFB b THEN c1 ELSE c2 FI) (IFB b' THEN c1' ELSE c2' FI).
 Proof.
   (* FILL IN HERE *) Admitted.
 (** [] *)
 
-(** *** *)
+(** **** 練習問題: ★★★ (CIf_congruence) *)
+Theorem CIf_congruence : forall b b' c1 c1' c2 c2',
+  bequiv b b' -> cequiv c1 c1' -> cequiv c2 c2' ->
+  cequiv (IFB b THEN c1 ELSE c2 FI)
+         (IFB b' THEN c1' ELSE c2' FI).
+Proof.
+  (* FILL IN HERE *) Admitted.
+(** [] *)
 
 (*  For example, here are two equivalent programs and a proof of their
     equivalence... *)
@@ -1008,35 +1008,30 @@ Example congruence_example:
        Y ::= ANum 42
      FI).
 Proof.
-  apply CSeq_congruence. 
-    apply refl_cequiv. 
+  apply CSeq_congruence.
+    apply refl_cequiv.
     apply CIf_congruence.
       apply refl_bequiv.
-      apply CAss_congruence. unfold aequiv. simpl. 
+      apply CAss_congruence. unfold aequiv. simpl.
         symmetry. apply minus_diag.
-      apply refl_cequiv. 
+      apply refl_cequiv.
 Qed.
 
 (* ####################################################### *)
 (*  * Program Transformations *)
 (** プログラムの変換 *)
 
-(* A _program transformation_ is a function that takes a program
-    as input and produces some variant of the program as its
-    output.  Compiler optimizations such as constant folding are
-    a canonical example, but there are many others. *)
+(*  A _program transformation_ is a function that takes a program as
+    input and produces some variant of the program as output.
+    Compiler optimizations such as constant folding are a canonical
+    example, but there are many others. *)
 (** プログラム変換(_program transformation_)とは、
     プログラムを入力とし、出力としてそのプログラムの何らかの変形を生成する関数です。
     定数畳み込みのようなコンパイラの最適化は標準的な例ですが、それ以外のものもたくさんあります。*)
 
 (* A program transformation is _sound_ if it preserves the
-    behavior of the original program. 
- 
-    We can define a notion of soundness for translations of
-    [aexp]s, [bexp]s, and [com]s. *)
-(** プログラム変換が健全(_sound_)とは、その変換が元のプログラムの振る舞いを保存することです。
-    
-    [aexp]、[bexp]、[com]の変換の健全性の概念を定義することができます。*)
+    behavior of the original program. *)
+(** プログラム変換が健全(_sound_)とは、その変換が元のプログラムの振る舞いを保存することです。*)
 
 Definition atrans_sound (atrans : aexp -> aexp) : Prop :=
   forall (a : aexp),
@@ -1067,26 +1062,29 @@ Fixpoint fold_constants_aexp (a : aexp) : aexp :=
   match a with
   | ANum n       => ANum n
   | AId i        => AId i
-  | APlus a1 a2  => 
-      match (fold_constants_aexp a1, fold_constants_aexp a2) with
-      | (ANum n1, ANum n2) => ANum (n1 + n2)
-      | (a1', a2') => APlus a1' a2'
-      end
-  | AMinus a1 a2 => 
-      match (fold_constants_aexp a1, fold_constants_aexp a2) with
-      | (ANum n1, ANum n2) => ANum (n1 - n2)
-      | (a1', a2') => AMinus a1' a2'
-      end
-  | AMult a1 a2  => 
-      match (fold_constants_aexp a1, fold_constants_aexp a2) with
-      | (ANum n1, ANum n2) => ANum (n1 * n2)
-      | (a1', a2') => AMult a1' a2'
-      end
+  | APlus a1 a2  =>
+    match (fold_constants_aexp a1, fold_constants_aexp a2)
+    with
+    | (ANum n1, ANum n2) => ANum (n1 + n2)
+    | (a1', a2') => APlus a1' a2'
+    end
+  | AMinus a1 a2 =>
+    match (fold_constants_aexp a1, fold_constants_aexp a2)
+    with
+    | (ANum n1, ANum n2) => ANum (n1 - n2)
+    | (a1', a2') => AMinus a1' a2'
+    end
+  | AMult a1 a2  =>
+    match (fold_constants_aexp a1, fold_constants_aexp a2)
+    with
+    | (ANum n1, ANum n2) => ANum (n1 * n2)
+    | (a1', a2') => AMult a1' a2'
+    end
   end.
 
 Example fold_aexp_ex1 :
-    fold_constants_aexp 
-      (AMult (APlus (ANum 1) (ANum 2)) (AId X)) 
+    fold_constants_aexp
+      (AMult (APlus (ANum 1) (ANum 2)) (AId X))
   = AMult (ANum 3) (AId X).
 Proof. reflexivity. Qed.
 
@@ -1101,46 +1099,53 @@ Proof. reflexivity. Qed.
     定義と証明が長くなるだけです。*)
 
 Example fold_aexp_ex2 :
-    fold_constants_aexp 
-      (AMinus (AId X) (APlus (AMult (ANum 0) (ANum 6)) (AId Y)))
+    fold_constants_aexp
+      (AMinus (AId X) (APlus (AMult (ANum 0) (ANum 6))
+                             (AId Y)))
   = AMinus (AId X) (APlus (ANum 0) (AId Y)).
 Proof. reflexivity. Qed.
 
-(** *** *)
 (*  Not only can we lift [fold_constants_aexp] to [bexp]s (in the
     [BEq] and [BLe] cases), we can also find constant _boolean_
-    expressions and reduce them in-place. *)
+    expressions and evaluate them in-place. *)
 (** ([BEq]と[BLe]の場合に)[fold_constants_aexp]を[bexp]
-    に持ち上げることができるだけでなく、定数「ブール」式をみつけてその場で置換することもできます。*)
+    に持ち上げることができるだけでなく、定数「ブール」式をみつけてその場で評価することもできます。*)
 
 Fixpoint fold_constants_bexp (b : bexp) : bexp :=
   match b with
   | BTrue        => BTrue
   | BFalse       => BFalse
-  | BEq a1 a2  => 
-      match (fold_constants_aexp a1, fold_constants_aexp a2) with
-      | (ANum n1, ANum n2) => if beq_nat n1 n2 then BTrue else BFalse
-      | (a1', a2') => BEq a1' a2'
-      end
-  | BLe a1 a2  => 
-      match (fold_constants_aexp a1, fold_constants_aexp a2) with
-      | (ANum n1, ANum n2) => if ble_nat n1 n2 then BTrue else BFalse
-      | (a1', a2') => BLe a1' a2'
-      end
-  | BNot b1  => 
-      match (fold_constants_bexp b1) with
-      | BTrue => BFalse
-      | BFalse => BTrue
-      | b1' => BNot b1'
-      end
-  | BAnd b1 b2  => 
-      match (fold_constants_bexp b1, fold_constants_bexp b2) with
-      | (BTrue, BTrue) => BTrue
-      | (BTrue, BFalse) => BFalse
-      | (BFalse, BTrue) => BFalse
-      | (BFalse, BFalse) => BFalse
-      | (b1', b2') => BAnd b1' b2'
-      end
+  | BEq a1 a2  =>
+    match (fold_constants_aexp a1, fold_constants_aexp a2)
+    with
+    | (ANum n1, ANum n2) =>
+        if beq_nat n1 n2 then BTrue else BFalse
+    | (a1', a2') =>
+        BEq a1' a2'
+    end
+  | BLe a1 a2  =>
+    match (fold_constants_aexp a1, fold_constants_aexp a2)
+    with
+    | (ANum n1, ANum n2) =>
+        if leb n1 n2 then BTrue else BFalse
+    | (a1', a2') =>
+        BLe a1' a2'
+    end
+  | BNot b1  =>
+    match (fold_constants_bexp b1) with
+    | BTrue => BFalse
+    | BFalse => BTrue
+    | b1' => BNot b1'
+    end
+  | BAnd b1 b2  =>
+    match (fold_constants_bexp b1, fold_constants_bexp b2)
+    with
+    | (BTrue, BTrue) => BTrue
+    | (BTrue, BFalse) => BFalse
+    | (BFalse, BTrue) => BFalse
+    | (BFalse, BFalse) => BFalse
+    | (b1', b2') => BAnd b1' b2'
+    end
   end.
 
 Example fold_bexp_ex1 :
@@ -1149,34 +1154,34 @@ Example fold_bexp_ex1 :
 Proof. reflexivity. Qed.
 
 Example fold_bexp_ex2 :
-    fold_constants_bexp 
-      (BAnd (BEq (AId X) (AId Y)) 
-            (BEq (ANum 0) 
-                 (AMinus (ANum 2) (APlus (ANum 1) (ANum 1)))))
+    fold_constants_bexp
+      (BAnd (BEq (AId X) (AId Y))
+            (BEq (ANum 0)
+                 (AMinus (ANum 2) (APlus (ANum 1)
+                                         (ANum 1)))))
   = BAnd (BEq (AId X) (AId Y)) BTrue.
 Proof. reflexivity. Qed.
 
-(** *** *)
 (*  To fold constants in a command, we apply the appropriate folding
     functions on all embedded expressions. *)
 (** コマンド内の定数を畳み込みするために、含まれるすべての式に対応する畳み込み関数を適用します。*)
 
 Fixpoint fold_constants_com (c : com) : com :=
   match c with
-  | SKIP      => 
+  | SKIP      =>
       SKIP
-  | i ::= a  => 
+  | i ::= a  =>
       CAss i (fold_constants_aexp a)
-  | c1 ;; c2  => 
+  | c1 ;; c2  =>
       (fold_constants_com c1) ;; (fold_constants_com c2)
-  | IFB b THEN c1 ELSE c2 FI => 
+  | IFB b THEN c1 ELSE c2 FI =>
       match fold_constants_bexp b with
       | BTrue => fold_constants_com c1
       | BFalse => fold_constants_com c2
-      | b' => IFB b' THEN fold_constants_com c1 
+      | b' => IFB b' THEN fold_constants_com c1
                      ELSE fold_constants_com c2 FI
       end
-  | WHILE b DO c END => 
+  | WHILE b DO c END =>
       match fold_constants_bexp b with
       | BTrue => WHILE BTrue DO SKIP END
       | BFalse => SKIP
@@ -1186,66 +1191,69 @@ Fixpoint fold_constants_com (c : com) : com :=
 
 (** *** *)
 Example fold_com_ex1 :
-  fold_constants_com 
+  fold_constants_com
     (* Original program: *)
     (X ::= APlus (ANum 4) (ANum 5);;
      Y ::= AMinus (AId X) (ANum 3);;
-     IFB BEq (AMinus (AId X) (AId Y)) (APlus (ANum 2) (ANum 4)) THEN
-       SKIP 
+     IFB BEq (AMinus (AId X) (AId Y))
+             (APlus (ANum 2) (ANum 4)) THEN
+       SKIP
      ELSE
        Y ::= ANum 0
      FI;;
-     IFB BLe (ANum 0) (AMinus (ANum 4) (APlus (ANum 2) (ANum 1))) THEN
+     IFB BLe (ANum 0)
+             (AMinus (ANum 4) (APlus (ANum 2) (ANum 1))) 
+     THEN
        Y ::= ANum 0
      ELSE
-       SKIP 
+       SKIP
      FI;;
-     WHILE BEq (AId Y) (ANum 0) DO 
-       X ::= APlus (AId X) (ANum 1) 
-     END) 
+     WHILE BEq (AId Y) (ANum 0) DO
+       X ::= APlus (AId X) (ANum 1)
+     END)
   = (* After constant folding: *)
     (X ::= ANum 9;;
      Y ::= AMinus (AId X) (ANum 3);;
      IFB BEq (AMinus (AId X) (AId Y)) (ANum 6) THEN
-       SKIP 
+       SKIP
      ELSE
-       (Y ::= ANum 0) 
+       (Y ::= ANum 0)
      FI;;
      Y ::= ANum 0;;
-     WHILE BEq (AId Y) (ANum 0) DO 
-       X ::= APlus (AId X) (ANum 1) 
+     WHILE BEq (AId Y) (ANum 0) DO
+       X ::= APlus (AId X) (ANum 1)
      END).
 Proof. reflexivity. Qed.
 
 (* ################################################### *)
-(* ** Soundness of Constant Folding *)
+(*  ** Soundness of Constant Folding *)
 (** ** 定数畳み込みの健全性 *)
 
-(* Now we need to show that what we've done is correct. *)
+(*  Now we need to show that what we've done is correct. *)
 (** 上でやったことが正しいことを示さなければなりません。*)
 
 (*  Here's the proof for arithmetic expressions: *)
 (** 算術式に対する証明です: *)
+
 Theorem fold_constants_aexp_sound :
   atrans_sound fold_constants_aexp.
 Proof.
   unfold atrans_sound. intros a. unfold aequiv. intros st.
-  aexp_cases (induction a) Case; simpl;
+  induction a; simpl;
     (* ANum and AId follow immediately *)
     try reflexivity;
     (* APlus, AMinus, and AMult follow from the IH
        and the observation that
-              aeval st (APlus a1 a2) 
-            = ANum ((aeval st a1) + (aeval st a2)) 
+              aeval st (APlus a1 a2)
+            = ANum ((aeval st a1) + (aeval st a2))
             = aeval st (ANum ((aeval st a1) + (aeval st a2)))
        (and similarly for AMinus/minus and AMult/mult) *)
     try (destruct (fold_constants_aexp a1);
          destruct (fold_constants_aexp a2);
          rewrite IHa1; rewrite IHa2; reflexivity). Qed.
 
-(* **** Exercise: 3 stars, optional (fold_bexp_BEq_informal)  *)
-(** **** 練習問題: ★★★, optional (fold_bexp_BEq_informal) *)
-(* Here is an informal proof of the [BEq] case of the soundness
+(** **** 練習問題: ★★★, optional (fold_bexp_Eq_informal) *)
+(*  Here is an informal proof of the [BEq] case of the soundness
     argument for boolean expression constant folding.  Read it
     carefully and compare it to the formal proof that follows.  Then
     fill in the [BLe] case of the formal proof (without looking at the
@@ -1258,62 +1266,83 @@ Proof.
    for all boolean expressions [b].  Proceed by induction on [b].  We
    show just the case where [b] has the form [BEq a1 a2].
 
-   In this case, we must show 
-       beval st (BEq a1 a2) 
+   In this case, we must show
+
+       beval st (BEq a1 a2)
      = beval st (fold_constants_bexp (BEq a1 a2)).
+
    There are two cases to consider:
 
      - First, suppose [fold_constants_aexp a1 = ANum n1] and
        [fold_constants_aexp a2 = ANum n2] for some [n1] and [n2].
 
        In this case, we have
-           fold_constants_bexp (BEq a1 a2) 
+
+           fold_constants_bexp (BEq a1 a2)
          = if beq_nat n1 n2 then BTrue else BFalse
+
        and
-           beval st (BEq a1 a2) 
+
+           beval st (BEq a1 a2)
          = beq_nat (aeval st a1) (aeval st a2).
+
        By the soundness of constant folding for arithmetic
        expressions (Lemma [fold_constants_aexp_sound]), we know
-           aeval st a1 
-         = aeval st (fold_constants_aexp a1) 
-         = aeval st (ANum n1) 
+
+           aeval st a1
+         = aeval st (fold_constants_aexp a1)
+         = aeval st (ANum n1)
          = n1
+
        and
-           aeval st a2 
-         = aeval st (fold_constants_aexp a2) 
-         = aeval st (ANum n2) 
+
+           aeval st a2
+         = aeval st (fold_constants_aexp a2)
+         = aeval st (ANum n2)
          = n2,
+
        so
-           beval st (BEq a1 a2) 
+
+           beval st (BEq a1 a2)
          = beq_nat (aeval a1) (aeval a2)
          = beq_nat n1 n2.
+
        Also, it is easy to see (by considering the cases [n1 = n2] and
        [n1 <> n2] separately) that
+
            beval st (if beq_nat n1 n2 then BTrue else BFalse)
          = if beq_nat n1 n2 then beval st BTrue else beval st BFalse
          = if beq_nat n1 n2 then true else false
          = beq_nat n1 n2.
+
        So
-           beval st (BEq a1 a2) 
+
+           beval st (BEq a1 a2)
          = beq_nat n1 n2.
          = beval st (if beq_nat n1 n2 then BTrue else BFalse),
-]]         
+
        as required.
 
      - Otherwise, one of [fold_constants_aexp a1] and
        [fold_constants_aexp a2] is not a constant.  In this case, we
        must show
-           beval st (BEq a1 a2) 
+
+           beval st (BEq a1 a2)
          = beval st (BEq (fold_constants_aexp a1)
                          (fold_constants_aexp a2)),
+
        which, by the definition of [beval], is the same as showing
-           beq_nat (aeval st a1) (aeval st a2) 
+
+           beq_nat (aeval st a1) (aeval st a2)
          = beq_nat (aeval st (fold_constants_aexp a1))
                    (aeval st (fold_constants_aexp a2)).
+
        But the soundness of constant folding for arithmetic
        expressions ([fold_constants_aexp_sound]) gives us
+
          aeval st a1 = aeval st (fold_constants_aexp a1)
          aeval st a2 = aeval st (fold_constants_aexp a2),
+
        completing the case.  []
 *)
 (** ここに、ブール式の定数畳み込みに関する健全性の議論の[BEq]の場合の非形式的証明を示します。
@@ -1375,7 +1404,7 @@ Proof.
          = beval st (BEq (fold_constants_aexp a1)
                          (fold_constants_aexp a2)),
        を示せば良い。
-       [beval]の定義から、これは     
+       [beval]の定義から、これは    
            beq_nat (aeval st a1) (aeval st a2)
          = beq_nat (aeval st (fold_constants_aexp a1))
                    (aeval st (fold_constants_aexp a2)).
@@ -1390,16 +1419,17 @@ Theorem fold_constants_bexp_sound:
   btrans_sound fold_constants_bexp.
 Proof.
   unfold btrans_sound. intros b. unfold bequiv. intros st.
-  bexp_cases (induction b) Case; 
+  induction b;
     (* BTrue and BFalse are immediate *)
-    try reflexivity. 
-  Case "BEq". 
-    (* Doing induction when there are a lot of constructors makes
-       specifying variable names a chore, but Coq doesn't always
-       choose nice variable names.  We can rename entries in the
-       context with the [rename] tactic: [rename a into a1] will
-       change [a] to [a1] in the current goal and context. *)
+    try reflexivity.
+  - (* BEq *)
     rename a into a1. rename a0 into a2. simpl.
+
+    (* (Doing induction when there are a lot of constructors makes
+        specifying variable names a chore, but Coq doesn't always
+        choose nice variable names.  We can rename entries in the
+        context with the [rename] tactic: [rename a into a1] will
+        change [a] to [a1] in the current goal and context.) *)
     remember (fold_constants_aexp a1) as a1' eqn:Heqa1'.
     remember (fold_constants_aexp a2) as a2' eqn:Heqa2'.
     replace (aeval st a1) with (aeval st a1') by
@@ -1407,50 +1437,55 @@ Proof.
     replace (aeval st a2) with (aeval st a2') by
        (subst a2'; rewrite <- fold_constants_aexp_sound; reflexivity).
     destruct a1'; destruct a2'; try reflexivity.
-      (* The only interesting case is when both a1 and a2 
-         become constants after folding *)
+
+      (* The only interesting case is when both a1 and a2
+          become constants after folding *)
       simpl. destruct (beq_nat n n0); reflexivity.
-  Case "BLe". 
+  - (* BLe *)
     (* FILL IN HERE *) admit.
-  Case "BNot". 
-    simpl. remember (fold_constants_bexp b) as b' eqn:Heqb'. 
+  - (* BNot *)
+    simpl. remember (fold_constants_bexp b) as b' eqn:Heqb'.
     rewrite IHb.
-    destruct b'; reflexivity. 
-  Case "BAnd". 
-    simpl. 
-    remember (fold_constants_bexp b1) as b1' eqn:Heqb1'. 
+    destruct b'; reflexivity.
+  - (* BAnd *)
+    simpl.
+    remember (fold_constants_bexp b1) as b1' eqn:Heqb1'.
     remember (fold_constants_bexp b2) as b2' eqn:Heqb2'.
     rewrite IHb1. rewrite IHb2.
-    destruct b1'; destruct b2'; reflexivity.  Qed.
+    destruct b1'; destruct b2'; reflexivity.
+(* FILL IN HERE *) Admitted.
 (** [] *)
 
-(* **** Exercise: 3 stars (fold_constants_com_sound) *)
 (** **** 練習問題: ★★★ (fold_constants_com_sound) *)
 (* Complete the [WHILE] case of the following proof. *)
 (** 次の証明の[WHILE]の場合を完成させなさい。*)
 
-Theorem fold_constants_com_sound : 
+Theorem fold_constants_com_sound :
   ctrans_sound fold_constants_com.
-Proof. 
-  unfold ctrans_sound. intros c. 
-  com_cases (induction c) Case; simpl.
-  Case "SKIP". apply refl_cequiv.
-  Case "::=". apply CAss_congruence. apply fold_constants_aexp_sound.
-  Case ";;". apply CSeq_congruence; assumption.
-  Case "IFB". 
-    assert (bequiv b (fold_constants_bexp b)).
-      SCase "Pf of assertion". apply fold_constants_bexp_sound.
+Proof.
+  unfold ctrans_sound. intros c.
+  induction c; simpl.
+  - (* SKIP *) apply refl_cequiv.
+  - (* ::= *) apply CAss_congruence.
+              apply fold_constants_aexp_sound.
+  - (* ;; *) apply CSeq_congruence; assumption.
+  - (* IFB *)
+    assert (bequiv b (fold_constants_bexp b)). {
+      apply fold_constants_bexp_sound. }
     destruct (fold_constants_bexp b) eqn:Heqb;
-      (* If the optimization doesn't eliminate the if, then the result
-         is easy to prove from the IH and fold_constants_bexp_sound *)
       try (apply CIf_congruence; assumption).
-    SCase "b always true".
+
+      (*  (If the optimization doesn't eliminate the if, then the
+          result is easy to prove from the IH and
+          [fold_constants_bexp_sound].) *)
+      (** もし最適化がifを削除しないならば、結果はIHと[fold_constants_bexp_sound]から直ちに証明出来ます。 *)
+    + (* b always true *)
       apply trans_cequiv with c1; try assumption.
       apply IFB_true; assumption.
-    SCase "b always false".
+    + (* b always false *)
       apply trans_cequiv with c2; try assumption.
       apply IFB_false; assumption.
-  Case "WHILE".
+  - (* WHILE *)
     (* FILL IN HERE *) Admitted.
 (** [] *)
 
@@ -1458,33 +1493,34 @@ Proof.
 (* *** Soundness of (0 + n) Elimination, Redux *)
 (** *** (0 + n)の消去の健全性、再び *)
 
-(* **** Exercise: 4 stars, optional (optimize_0plus) *)
 (** **** 練習問題: ★★★★, optional (optimize_0plus) *)
 (* Recall the definition [optimize_0plus] from Imp.v:
+
     Fixpoint optimize_0plus (e:aexp) : aexp :=
       match e with
-      | ANum n => 
+      | ANum n =>
           ANum n
-      | APlus (ANum 0) e2 => 
+      | APlus (ANum 0) e2 =>
           optimize_0plus e2
-      | APlus e1 e2 => 
+      | APlus e1 e2 =>
           APlus (optimize_0plus e1) (optimize_0plus e2)
-      | AMinus e1 e2 => 
+      | AMinus e1 e2 =>
           AMinus (optimize_0plus e1) (optimize_0plus e2)
-      | AMult e1 e2 => 
+      | AMult e1 e2 =>
           AMult (optimize_0plus e1) (optimize_0plus e2)
       end.
    Note that this function is defined over the old [aexp]s,
    without states.
 
    Write a new version of this function that accounts for variables,
-   and analogous ones for [bexp]s and commands:
+   plus analogous ones for [bexp]s and commands:
+
      optimize_0plus_aexp
      optimize_0plus_bexp
      optimize_0plus_com
    Prove that these three functions are sound, as we did for
-   [fold_constants_*].  (Make sure you use the congruence lemmas in
-   the proof of [optimize_0plus_com] -- otherwise it will be _long_!)
+   [fold_constants_*].  Make sure you use the congruence lemmas in
+   the proof of [optimize_0plus_com] -- otherwise it will be _long_!
 
    Then define an optimizer on commands that first folds
    constants (using [fold_constants_com]) and then eliminates [0 + n]
@@ -1497,15 +1533,15 @@ Proof.
 (** Imp_J.vの[optimize_0plus]の定義をふり返ります。
     Fixpoint optimize_0plus (e:aexp) : aexp :=
       match e with
-      | ANum n => 
+      | ANum n =>
           ANum n
-      | APlus (ANum 0) e2 => 
+      | APlus (ANum 0) e2 =>
           optimize_0plus e2
-      | APlus e1 e2 => 
+      | APlus e1 e2 =>
           APlus (optimize_0plus e1) (optimize_0plus e2)
-      | AMinus e1 e2 => 
+      | AMinus e1 e2 =>
           AMinus (optimize_0plus e1) (optimize_0plus e2)
-      | AMult e1 e2 => 
+      | AMult e1 e2 =>
           AMult (optimize_0plus e1) (optimize_0plus e2)
       end.
    この関数は、[aexp]の上で定義されていて、状態を扱わないことに注意します。
@@ -1519,7 +1555,7 @@ Proof.
 ]]
    これらの関数の健全性を、[fold_constants_*]について行ったのと同様に証明しなさい。
    [optimize_0plus_com]の証明においては、合同性補題を確実に使いなさい
-   (そうしなければ証明はとても長くなるでしょう!)。
+   そうしなければ証明はとても長くなるでしょう!
 
    次に、コマンドに対して次の処理を行う最適化関数を定義しなさい。行うべき処理は、
    まず定数畳み込みを([fold_constants_com]を使って)行い、
@@ -1536,14 +1572,16 @@ Proof.
 (* * Proving That Programs Are _Not_ Equivalent *)
 (** * プログラムが同値でないことを証明する *)
 
-(* Suppose that [c1] is a command of the form [X ::= a1; Y ::= a2]
+(*  Suppose that [c1] is a command of the form [X ::= a1; Y ::= a2]
     and [c2] is the command [X ::= a1; Y ::= a2'], where [a2'] is
     formed by substituting [a1] for all occurrences of [X] in [a2].
     For example, [c1] and [c2] might be:
-       c1  =  (X ::= 42 + 53;; 
+
+       c1  =  (X ::= 42 + 53;;
                Y ::= Y + X)
-       c2  =  (X ::= 42 + 53;; 
+       c2  =  (X ::= 42 + 53;;
                Y ::= Y + (42 + 53))
+
     Clearly, this _particular_ [c1] and [c2] are equivalent.  Is this
     true in general? *)
 (** [c1]が[X ::= a1; Y ::= a2]という形のコマンドで、
@@ -1552,7 +1590,7 @@ Proof.
     例えば、[c1]と[c2]は次のようなものです。
        c1  =  (X ::= 42 + 53;
                Y ::= Y + X)
-       c2  =  (X ::= 42 + 53;; 
+       c2  =  (X ::= 42 + 53;;
                Y ::= Y + (42 + 53))
     明らかに、この例の場合は[c1]と[c2]は同値です。
     しかし、一般にそうだと言えるでしょうか？ *)
@@ -1571,19 +1609,25 @@ Proof.
 
 Fixpoint subst_aexp (i : id) (u : aexp) (a : aexp) : aexp :=
   match a with
-  | ANum n       => ANum n
-  | AId i'       => if eq_id_dec i i' then u else AId i'
-  | APlus a1 a2  => APlus (subst_aexp i u a1) (subst_aexp i u a2)
-  | AMinus a1 a2 => AMinus (subst_aexp i u a1) (subst_aexp i u a2)
-  | AMult a1 a2  => AMult (subst_aexp i u a1) (subst_aexp i u a2)
+  | ANum n       =>
+      ANum n
+  | AId i'       =>
+      if beq_id i i' then u else AId i'
+  | APlus a1 a2  =>
+      APlus (subst_aexp i u a1) (subst_aexp i u a2)
+  | AMinus a1 a2 =>
+      AMinus (subst_aexp i u a1) (subst_aexp i u a2)
+  | AMult a1 a2  =>
+      AMult (subst_aexp i u a1) (subst_aexp i u a2)
   end.
 
 Example subst_aexp_ex :
-  subst_aexp X (APlus (ANum 42) (ANum 53)) (APlus (AId Y) (AId X)) =
-  (APlus (AId Y) (APlus (ANum 42) (ANum 53))).
+  subst_aexp X (APlus (ANum 42) (ANum 53))
+             (APlus (AId Y) (AId X))
+= (APlus (AId Y) (APlus (ANum 42) (ANum 53))).
 Proof. reflexivity.  Qed.
 
-(* And here is the property we are interested in, expressing the
+(*  And here is the property we are interested in, expressing the
     claim that commands [c1] and [c2] as described above are
     always equivalent.  *)
 (** そして次が、興味対象の性質です。
@@ -1593,34 +1637,46 @@ Definition subst_equiv_property := forall i1 i2 a1 a2,
   cequiv (i1 ::= a1;; i2 ::= a2)
          (i1 ::= a1;; i2 ::= subst_aexp i1 a1 a2).
 
-(** *** *)
-(*  Sadly, the property does _not_ always hold. 
+(*  Sadly, the property does _not_ always hold.
 
     _Theorem_: It is not the case that, for all [i1], [i2], [a1],
     and [a2],
+
          cequiv (i1 ::= a1;; i2 ::= a2)
                 (i1 ::= a1;; i2 ::= subst_aexp i1 a1 a2).
-]] 
+
     _Proof_: Suppose, for a contradiction, that for all [i1], [i2],
     [a1], and [a2], we have
-      cequiv (i1 ::= a1;; i2 ::= a2) 
+
+      cequiv (i1 ::= a1;; i2 ::= a2)
              (i1 ::= a1;; i2 ::= subst_aexp i1 a1 a2).
+
     Consider the following program:
+
          X ::= APlus (AId X) (ANum 1);; Y ::= AId X
+
     Note that
+
          (X ::= APlus (AId X) (ANum 1);; Y ::= AId X)
-         / empty_state || st1,
+         / empty_state \\ st1,
+
     where [st1 = { X |-> 1, Y |-> 1 }].
 
     By our assumption, we know that
+
         cequiv (X ::= APlus (AId X) (ANum 1);; Y ::= AId X)
                (X ::= APlus (AId X) (ANum 1);; Y ::= APlus (AId X) (ANum 1))
+
     so, by the definition of [cequiv], we have
+
         (X ::= APlus (AId X) (ANum 1);; Y ::= APlus (AId X) (ANum 1))
-        / empty_state || st1.
+        / empty_state \\ st1.
+
     But we can also derive
+
         (X ::= APlus (AId X) (ANum 1);; Y ::= APlus (AId X) (ANum 1))
-        / empty_state || st2,
+        / empty_state \\ st2,
+
     where [st2 = { X |-> 1, Y |-> 2 }].  Note that [st1 <> st2]; this
     is a contradiction, since [ceval] is deterministic!  [] *)
 (** 残念ながら、この性質は、常には成立「しません」。
@@ -1632,14 +1688,14 @@ Definition subst_equiv_property := forall i1 i2 a1 a2,
 ]]
 
     「証明」:仮にすべての[i1], [i2], [a1], [a2]について
-      cequiv (i1 ::= a1;; i2 ::= a2) 
+      cequiv (i1 ::= a1;; i2 ::= a2)
              (i1 ::= a1;; i2 ::= subst_aexp i1 a1 a2).
     が成立するとする。
     次のプログラムを考える:
          X ::= APlus (AId X) (ANum 1);; Y ::= AId X
     次のことに注意する:
          (X ::= APlus (AId X) (ANum 1);; Y ::= AId X)
-         / empty_state || st1,
+         / empty_state \\ st1,
     ここで [st1 = { X |-> 1, Y |-> 1 }]である。
 
     仮定より、次が言える:
@@ -1647,15 +1703,15 @@ Definition subst_equiv_property := forall i1 i2 a1 a2,
                (X ::= APlus (AId X) (ANum 1);; Y ::= APlus (AId X) (ANum 1))
     すると、[cequiv]の定義より、次が言える:
         (X ::= APlus (AId X) (ANum 1);; Y ::= APlus (AId X) (ANum 1))
-        / empty_state || st1.
+        / empty_state \\ st1.
     しかし次のことも言える:
         (X ::= APlus (AId X) (ANum 1);; Y ::= APlus (AId X) (ANum 1))
-        / empty_state || st2,
+        / empty_state \\ st2,
     ただし[st2 = { X |-> 1, Y |-> 2 }]である。
     [st1 <> st2]に注意すると、これは[ceval]が決定性を持つことに矛盾する!
       [] *)
 
-Theorem subst_inequiv : 
+Theorem subst_inequiv :
   ~ subst_equiv_property.
 Proof.
   unfold subst_equiv_property.
@@ -1664,10 +1720,10 @@ Proof.
   (* Here is the counterexample: assuming that [subst_equiv_property]
      holds allows us to prove that these two programs are
      equivalent... *)
-  remember (X ::= APlus (AId X) (ANum 1);
+  remember (X ::= APlus (AId X) (ANum 1);;
             Y ::= AId X)
       as c1.
-  remember (X ::= APlus (AId X) (ANum 1);
+  remember (X ::= APlus (AId X) (ANum 1);;
             Y ::= APlus (AId X) (ANum 1))
       as c2.
   assert (cequiv c1 c2) by (subst; apply Contra).
@@ -1676,12 +1732,12 @@ Proof.
      in two different final states:
         st1 = {X |-> 1, Y |-> 1}
         st2 = {X |-> 1, Y |-> 2}. *)
-  remember (update (update empty_state X 1) Y 1) as st1.
-  remember (update (update empty_state X 1) Y 2) as st2.
-  assert (H1: c1 / empty_state || st1);
-  assert (H2: c2 / empty_state || st2);
+  remember (t_update (t_update empty_state X 1) Y 1) as st1.
+  remember (t_update (t_update empty_state X 1) Y 2) as st2.
+  assert (H1: c1 / empty_state \\ st1);
+  assert (H2: c2 / empty_state \\ st2);
   try (subst;
-       apply E_Seq with (st' := (update empty_state X 1));
+       apply E_Seq with (st' := (t_update empty_state X 1));
        apply E_Ass; reflexivity).
   apply H in H1.
 
@@ -1693,9 +1749,8 @@ Proof.
     by (rewrite Hcontra; reflexivity).
   subst. inversion Hcontra'.  Qed.
 
-(* **** Exercise: 4 stars (better_subst_equiv) *)
 (** **** 練習問題: ★★★★ (better_subst_equiv) *)
-(* The equivalence we had in mind above was not complete nonsense --
+(*  The equivalence we had in mind above was not complete nonsense --
     it was actually almost right.  To make it correct, we just need to
     exclude the case where the variable [X] occurs in the
     right-hand-side of the first assignment statement. *)
@@ -1721,11 +1776,11 @@ Inductive var_not_used_in_aexp (X:id) : aexp -> Prop :=
 
 Lemma aeval_weakening : forall i st a ni,
   var_not_used_in_aexp i a ->
-  aeval (update st i ni) a = aeval st a.
+  aeval (t_update st i ni) a = aeval st a.
 Proof.
   (* FILL IN HERE *) Admitted.
 
-(* Using [var_not_used_in_aexp], formalize and prove a correct verson
+(*  Using [var_not_used_in_aexp], formalize and prove a correct verson
     of [subst_equiv_property]. *)
 (** [var_not_used_in_aexp]を使って、[subst_equiv_property]の正しいバージョンを形式化し、
     証明しなさい。*)
@@ -1733,16 +1788,17 @@ Proof.
 (* FILL IN HERE *)
 (** [] *)
 
-(* **** Exercise: 3 stars, recommended (inequiv_exercise)  *)
 (** **** 練習問題: ★★★, recommended (inequiv_exercise)  *)
 (*  Prove that an infinite loop is not equivalent to [SKIP] *)
 (** 無限ループは、[SKIP]と等しくないことを証明しなさい *)
-Theorem inequiv_exercise: 
+
+Theorem inequiv_exercise:
   ~ cequiv (WHILE BTrue DO SKIP END) SKIP.
 Proof.
   (* FILL IN HERE *) Admitted.
 (** [] *)
 
+(* ################################################################## *)
 (** * Extended exercise: Non-deterministic Imp *)
 
 (** As we have seen (in theorem [ceval_deterministic] in the Imp
@@ -1752,30 +1808,34 @@ Proof.
     languages (such as C and its relatives), the order in which
     function arguments are evaluated is unspecified.  The program
     fragment
+
       x = 0;;
       f(++x, x)
+
     might call [f] with arguments [(1, 0)] or [(1, 1)], depending how
     the compiler chooses to order things.  This can be a little
     confusing for programmers, but it gives the compiler writer useful
     freedom.
 
     In this exercise, we will extend Imp with a simple
-    non-deterministic command and study how this change affects
+    nondeterministic command and study how this change affects
     program equivalence.  The new command has the syntax [HAVOC X],
     where [X] is an identifier. The effect of executing [HAVOC X] is
     to assign an _arbitrary_ number to the variable [X],
-    non-deterministically. For example, after executing the program:
+    nondeterministically. For example, after executing the program:
+
       HAVOC Y;;
       Z ::= Y * 2
+
     the value of [Y] can be any number, while the value of [Z] is
     twice that of [Y] (so [Z] is always even). Note that we are not
     saying anything about the _probabilities_ of the outcomes -- just
     that there are (infinitely) many different outcomes that can
-    possibly happen after executing this non-deterministic code.
+    possibly happen after executing this nondeterministic code.
 
-    In a sense a variable on which we do [HAVOC] roughly corresponds
-    to an unitialized variable in the C programming language. After
-    the [HAVOC] the variable holds a fixed but arbitrary number.  Most
+    In a sense, a variable on which we do [HAVOC] roughly corresponds
+    to an unitialized variable in a low-level language like C.  After
+    the [HAVOC], the variable holds a fixed but arbitrary number.  Most
     sources of nondeterminism in language definitions are there
     precisely because programmers don't care which choice is made (and
     so it is good to leave it open to the compiler to choose whichever
@@ -1785,8 +1845,8 @@ Proof.
 
 Module Himp.
 
-(** To formalize the language, we first add a clause to the definition of
-   commands. *)
+(** To formalize Himp, we first add a clause to the definition of
+    commands. *)
 
 Inductive com : Type :=
   | CSkip : com
@@ -1795,11 +1855,6 @@ Inductive com : Type :=
   | CIf : bexp -> com -> com -> com
   | CWhile : bexp -> com -> com
   | CHavoc : id -> com.                (* <---- new *)
-
-Tactic Notation "com_cases" tactic(first) ident(c) :=
-  first;
-  [ Case_aux c "SKIP" | Case_aux c "::=" | Case_aux c ";;"
-  | Case_aux c "IFB" | Case_aux c "WHILE" | Case_aux c "HAVOC" ].
 
 Notation "'SKIP'" :=
   CSkip.
@@ -1819,48 +1874,47 @@ Notation "'HAVOC' l" := (CHavoc l) (at level 60).
    semantics. What rule(s) must be added to the definition of [ceval]
    to formalize the behavior of the [HAVOC] command? *)
 
-Reserved Notation "c1 '/' st '||' st'" (at level 40, st at level 39).
+Reserved Notation "c1 '/' st '\\' st'"
+                  (at level 40, st at level 39).
 
 Inductive ceval : com -> state -> state -> Prop :=
-  | E_Skip : forall st : state, SKIP / st || st
+  | E_Skip : forall st : state, SKIP / st \\ st
   | E_Ass : forall (st : state) (a1 : aexp) (n : nat) (X : id),
-            aeval st a1 = n -> (X ::= a1) / st || update st X n
+      aeval st a1 = n ->
+      (X ::= a1) / st \\ t_update st X n
   | E_Seq : forall (c1 c2 : com) (st st' st'' : state),
-            c1 / st || st' -> c2 / st' || st'' -> (c1 ;; c2) / st || st''
+      c1 / st \\ st' ->
+      c2 / st' \\ st'' ->
+      (c1 ;; c2) / st \\ st''
   | E_IfTrue : forall (st st' : state) (b1 : bexp) (c1 c2 : com),
-               beval st b1 = true ->
-               c1 / st || st' -> (IFB b1 THEN c1 ELSE c2 FI) / st || st'
+      beval st b1 = true ->
+      c1 / st \\ st' ->
+      (IFB b1 THEN c1 ELSE c2 FI) / st \\ st'
   | E_IfFalse : forall (st st' : state) (b1 : bexp) (c1 c2 : com),
-                beval st b1 = false ->
-                c2 / st || st' -> (IFB b1 THEN c1 ELSE c2 FI) / st || st'
+      beval st b1 = false ->
+      c2 / st \\ st' ->
+      (IFB b1 THEN c1 ELSE c2 FI) / st \\ st'
   | E_WhileEnd : forall (b1 : bexp) (st : state) (c1 : com),
-                 beval st b1 = false -> (WHILE b1 DO c1 END) / st || st
+      beval st b1 = false -> 
+      (WHILE b1 DO c1 END) / st \\ st
   | E_WhileLoop : forall (st st' st'' : state) (b1 : bexp) (c1 : com),
-                  beval st b1 = true ->
-                  c1 / st || st' ->
-                  (WHILE b1 DO c1 END) / st' || st'' ->
-                  (WHILE b1 DO c1 END) / st || st''
+      beval st b1 = true ->
+      c1 / st \\ st' ->
+      (WHILE b1 DO c1 END) / st' \\ st'' ->
+      (WHILE b1 DO c1 END) / st \\ st''
 (* FILL IN HERE *)
 
-  where "c1 '/' st '||' st'" := (ceval c1 st st').
-
-Tactic Notation "ceval_cases" tactic(first) ident(c) :=
-  first;
-  [ Case_aux c "E_Skip" | Case_aux c "E_Ass" | Case_aux c "E_Seq"
-  | Case_aux c "E_IfTrue" | Case_aux c "E_IfFalse"
-  | Case_aux c "E_WhileEnd" | Case_aux c "E_WhileLoop"
-(* FILL IN HERE *)
-].
+  where "c1 '/' st '\\' st'" := (ceval c1 st st').
 
 (** As a sanity check, the following claims should be provable for
-   your definition: *)
+    your definition: *)
 
-Example havoc_example1 : (HAVOC X) / empty_state || update empty_state X 0.
+Example havoc_example1 : (HAVOC X) / empty_state \\ t_update empty_state X 0.
 Proof.
 (* FILL IN HERE *) Admitted.
 
 Example havoc_example2 :
-  (SKIP;; HAVOC Z) / empty_state || update empty_state Z 42.
+  (SKIP;; HAVOC Z) / empty_state \\ t_update empty_state Z 42.
 Proof.
 (* FILL IN HERE *) Admitted.
 (** [] *)
@@ -1868,11 +1922,11 @@ Proof.
 (** Finally, we repeat the definition of command equivalence from above: *)
 
 Definition cequiv (c1 c2 : com) : Prop := forall st st' : state,
-  c1 / st || st' <-> c2 / st || st'.
+  c1 / st \\ st' <-> c2 / st \\ st'.
 
-(** This definition still makes perfect sense in the case of always
-    terminating programs, so let's apply it to prove some
-    non-deterministic programs equivalent or non-equivalent. *)
+(*  Let's apply this definition to prove some nondeterministic
+    programs equivalent / inequivalent. *)
+(** この定義を非決定性プログラムの同値、非同値の証明に適用してみましょう。*)
 
 (** **** Exercise: 3 stars (havoc_swap)  *)
 (** Are the following two programs equivalent? *)
@@ -1914,17 +1968,18 @@ Proof. (* FILL IN HERE *) Admitted.
     subtle consequences on programs that may loop forever.  What
     [cequiv] says is that the set of possible _terminating_ outcomes
     of two equivalent programs is the same. However, in a language
-    with non-determinism, like Himp, some programs always terminate,
+    with nondeterminism, like Himp, some programs always terminate,
     some programs always diverge, and some programs can
-    non-deterministically terminate in some runs and diverge in
+    nondeterministically terminate in some runs and diverge in
     others. The final part of the following exercise illustrates this
     phenomenon.
 *)
 
-(** **** Exercise: 5 stars, advanced (p1_p2_equiv)  *)
-(** Prove that p1 and p2 are equivalent. In this and the following
+(** **** 練習問題: ★★★★★, advanced (p1_p2_equiv)  *)
+(*  Prove that [p1] and [p2] are equivalent. In this and the following
     exercises, try to understand why the [cequiv] definition has the
     behavior it has on these examples. *)
+(** [p1]と[p2]が同値であることを証明しなさい。これと次の練習問題で、なぜ[cequiv]の定義がこれらの例において同じふるまいをするかを理解しなさい *)
 
 Definition p1 : com :=
   WHILE (BNot (BEq (AId X) (ANum 0))) DO
@@ -1937,22 +1992,21 @@ Definition p2 : com :=
     SKIP
   END.
 
-
 (** Intuitively, the programs have the same termination
     behavior: either they loop forever, or they terminate in the
     same state they started in.  We can capture the termination
-    behavior of p1 and p2 individually with these lemmas: *)
+    behavior of [p1] and [p2] individually with these lemmas: *)
 
 Lemma p1_may_diverge : forall st st', st X <> 0 ->
-  ~ p1 / st || st'.
+  ~ p1 / st \\ st'.
 Proof. (* FILL IN HERE *) Admitted.
 
 Lemma p2_may_diverge : forall st st', st X <> 0 ->
-  ~ p2 / st || st'.
+  ~ p2 / st \\ st'.
 Proof.
 (* FILL IN HERE *) Admitted.
 
-(** You should use these lemmas to prove that p1 and p2 are actually
+(** You should use these lemmas to prove that [p1] and [p2] are actually
     equivalent. *)
 
 Theorem p1_p2_equiv : cequiv p1 p2.
@@ -1960,7 +2014,6 @@ Proof. (* FILL IN HERE *) Admitted.
 (** [] *)
 
 (** **** Exercise: 4 stars, advanced (p3_p4_inquiv)  *)
-
 (** Prove that the following programs are _not_ equivalent. *)
 
 Definition p3 : com :=
@@ -1997,261 +2050,21 @@ Proof. (* FILL IN HERE *) Admitted.
 End Himp.
 
 (* ####################################################### *)
-(* * Doing Without Extensionality (Optional) *)
-(** * 外延性を使わずに行う (Optional) *)
-
-(* Purists might object to using the [functional_extensionality]
-    axiom.  In general, it can be quite dangerous to add axioms,
-    particularly several at once (as they may be mutually
-    inconsistent). In fact, [functional_extensionality] and
-    [excluded_middle] can both be assumed without any problems, but
-    some Coq users prefer to avoid such "heavyweight" general
-    techniques, and instead craft solutions for specific problems that
-    stay within Coq's standard logic.
-
-    For our particular problem here, rather than extending the
-    definition of equality to do what we want on functions
-    representing states, we could instead give an explicit notion of
-    _equivalence_ on states.  For example: *)
-(** 純粋主義者は、[functional_extensionality]を使うことに不服かもしれません。
-    一般に、公理を追加することは非常に危険です。
-    特に、一度にいくつも追加するときは(追加するものが相互に矛盾することもあるため)
-    そうです。
-    実際は、[functional_extensionality]と[excluded_middle]
-    は両者とも何の問題もなく導入できます。
-    しかし、Coqユーザの中には、このような「ヘビーウェイト」の一般テクニックを避け、
-    Coqの標準論理の中で特定の問題のために技巧的解法を使うことを選びたい人もいるでしょう。
-
-    ここで扱っている問題に特定するなら、
-    状態を表現している関数についてやりたいことをやるために等しさの定義を拡張するより、
-    状態の同値(_equivalence_)の概念を明示的に与えることもできたかもしれません。
-    例えば: *)
-
-Definition stequiv (st1 st2 : state) : Prop :=
-  forall (X:id), st1 X = st2 X.
-
-Notation "st1 '~' st2" := (stequiv st1 st2) (at level 30).
-
-(* It is easy to prove that [stequiv] is an _equivalence_ (i.e., it
-   is reflexive, symmetric, and transitive), so it partitions the set
-   of all states into equivalence classes. *)
-(** [stequiv]が同値関係(_equivalence_、 つまり、反射的、対称的、推移的関係)
-    であることを証明することは容易です。この同値関係により、
-    すべての状態の集合は同値類に分割されます。*)
-
-(* **** Exercise: 1 star, optional (stequiv_refl) *)
-(** **** 練習問題: ★, optional (stequiv_refl) *)
-Lemma stequiv_refl : forall (st : state),
-  st ~ st.
-Proof.
-  (* FILL IN HERE *) Admitted.
-(** [] *)
-
-(* **** Exercise: 1 star, optional (stequiv_sym) *)
-(** **** 練習問題: ★, optional (stequiv_sym) *)
-Lemma stequiv_sym : forall (st1 st2 : state),
-  st1 ~ st2 ->
-  st2 ~ st1.
-Proof.
-  (* FILL IN HERE *) Admitted.
-(** [] *)
-
-(* **** Exercise: 1 star, optional (stequiv_trans) *)
-(** **** 練習問題: ★, optional (stequiv_trans) *)
-Lemma stequiv_trans : forall (st1 st2 st3 : state), 
-  st1 ~ st2 -> 
-  st2 ~ st3 -> 
-  st1 ~ st3.
-Proof.  
-  (* FILL IN HERE *) Admitted.
-(** [] *)
-
-(* Another useful fact... *)
-(** 別の有用な事実です... *)
-(* **** Exercise: 1 star, optional (stequiv_update) *)
-(** **** 練習問題: ★, optional (stequiv_update) *)
-Lemma stequiv_update : forall (st1 st2 : state),
-  st1 ~ st2 -> 
-  forall (X:id) (n:nat),
-  update st1 X n ~ update st2 X n. 
-Proof.
-  (* FILL IN HERE *) Admitted.
-(** [] *)
-
-(* It is then straightforward to show that [aeval] and [beval] behave
-    uniformly on all members of an equivalence class: *)
-(** [aeval]と[beval]が同値類のすべての要素に対して同じように振る舞うことは、
-    ここからストレートに証明できます: *)
-
-(* **** Exercise: 2 stars, optional (stequiv_aeval) *)
-(** **** 練習問題: ★★, optional (stequiv_aeval) *)
-Lemma stequiv_aeval : forall (st1 st2 : state), 
-  st1 ~ st2 ->
-  forall (a:aexp), aeval st1 a = aeval st2 a. 
-Proof.
-  (* FILL IN HERE *) Admitted.
-(** [] *)
-
-(* **** Exercise: 2 stars, optional (stequiv_beval) *)
-(** **** 練習問題: ★★, optional (stequiv_beval) *)
-Lemma stequiv_beval : forall (st1 st2 : state), 
-  st1 ~ st2 ->
-  forall (b:bexp), beval st1 b = beval st2 b. 
-Proof.
-  (* FILL IN HERE *) Admitted.
-(** [] *)
-
-(* We can also characterize the behavior of [ceval] on equivalent
-    states (this result is a bit more complicated to write down
-    because [ceval] is a relation). *)
-(** 同値である状態の面から[ceval]の振る舞いを特徴づけることもできます
-    ([ceval]は関係なので、この結果を書き下すのはもうちょっと複雑です)。 *)
-
-Lemma stequiv_ceval: forall (st1 st2 : state),
-  st1 ~ st2 ->
-  forall (c: com) (st1': state),
-    (c / st1 || st1') ->
-    exists st2' : state,
-    ((c / st2 || st2') /\  st1' ~ st2').
-Proof.
-  intros st1 st2 STEQV c st1' CEV1. generalize dependent st2. 
-  induction CEV1; intros st2 STEQV.  
-  Case "SKIP".
-    exists st2. split.  
-      constructor. 
-      assumption.
-  Case ":=".
-    exists (update st2 x n). split. 
-       constructor.  rewrite <- H. symmetry.  apply stequiv_aeval. 
-       assumption. apply stequiv_update.  assumption.
-  Case ";".
-    destruct (IHCEV1_1 st2 STEQV) as [st2' [P1 EQV1]].
-    destruct (IHCEV1_2 st2' EQV1) as [st2'' [P2 EQV2]]. 
-    exists st2''.  split.
-      apply E_Seq with st2';  assumption. 
-      assumption.
-  Case "IfTrue".
-    destruct (IHCEV1 st2 STEQV) as [st2' [P EQV]].
-    exists st2'.  split. 
-      apply E_IfTrue.  rewrite <- H. symmetry. apply stequiv_beval. 
-      assumption. assumption. assumption.
-  Case "IfFalse".
-    destruct (IHCEV1 st2 STEQV) as [st2' [P EQV]].
-    exists st2'. split. 
-     apply E_IfFalse. rewrite <- H. symmetry. apply stequiv_beval. 
-     assumption.  assumption. assumption.
-  Case "WhileEnd".
-    exists st2. split.
-      apply E_WhileEnd. rewrite <- H. symmetry. apply stequiv_beval. 
-      assumption. assumption. 
-  Case "WhileLoop".
-    destruct (IHCEV1_1 st2 STEQV) as [st2' [P1 EQV1]].
-    destruct (IHCEV1_2 st2' EQV1) as [st2'' [P2 EQV2]].
-    exists st2''. split. 
-      apply E_WhileLoop with st2'.  rewrite <- H. symmetry. 
-      apply stequiv_beval. assumption. assumption. assumption.
-      assumption.
-Qed.
-
-(* Now we need to redefine [cequiv] to use [~] instead of [=].  It is
-    not completely trivial to do this in a way that keeps the
-    definition simple and symmetric, but here is one approach (thanks
-    to Andrew McCreight). We first define a looser variant of [||]
-    that "folds in" the notion of equivalence. *)
-(** ここで[cequiv]を[=]の代わりに[~]を使って再定義する必要があります。
-    定義の簡潔さと対称性を保ったまま再定義するのは、それほど自明なことではありません。
-    しかしその方法はあります(Andrew McCreightに感謝します)。
-    最初に[||]のより緩いバージョンを定義します。
-    これは同値概念の中に「畳み込まれ」ます。*)
-
-Reserved Notation "c1 '/' st '||'' st'" (at level 40, st at level 39).
-
-Inductive ceval' : com -> state -> state -> Prop :=
-  | E_equiv : forall c st st' st'',
-    c / st || st' -> 
-    st' ~ st'' ->
-    c / st ||' st''
-  where   "c1 '/' st '||'' st'" := (ceval' c1 st st').
-
-(* Now the revised definition of [cequiv'] looks familiar: *)
-(** すると[cequiv']の新しい定義は馴染みのあるものになります: *)
-
-Definition cequiv' (c1 c2 : com) : Prop :=
-  forall (st st' : state),
-    (c1 / st ||' st') <-> (c2 / st ||' st').
-
-(* A sanity check shows that the original notion of command
-   equivalence is at least as strong as this new one.  (The converse
-   is not true, naturally.) *)
-(** もとのコマンド同値の概念が、新しいものと同じ強さかそれより強いことをサニティチェックします。
-    (その逆は当然成立しません。) *)
-
-Lemma cequiv__cequiv' : forall (c1 c2: com),
-  cequiv c1 c2 -> cequiv' c1 c2.
-Proof. 
-  unfold cequiv, cequiv'; split; intros. 
-    inversion H0 ; subst.  apply E_equiv with st'0.  
-    apply (H st st'0); assumption. assumption. 
-    inversion H0 ; subst.  apply E_equiv with st'0.  
-    apply (H st st'0). assumption. assumption.
-Qed.
-
-(* **** Exercise: 2 stars, optional (identity_assignment') *)
-(** **** 練習問題: ★★, optional (identity_assignment') *)
-(* Finally, here is our example once more... (You can complete the
-    proof.) *)
-(** 最後にもとの例を再度扱います... (証明を完成しなさい。) *)
-
-Example identity_assignment' :
-  cequiv' SKIP (X ::= AId X).
-Proof.
-    unfold cequiv'.  intros.  split; intros. 
-    Case "->".
-      inversion H; subst; clear H. inversion H0; subst.   
-      apply E_equiv with (update st'0 X (st'0 X)). 
-      constructor. reflexivity.  apply stequiv_trans with st'0.  
-      unfold stequiv. intros. apply update_same. 
-      reflexivity. assumption. 
-    Case "<-".  
-      (* FILL IN HERE *) Admitted.
-(** [] *)
-
-(* On the whole, this explicit equivalence approach is considerably
-    harder to work with than relying on functional
-    extensionality. (Coq does have an advanced mechanism called
-    "setoids" that makes working with equivalences somewhat easier, by
-    allowing them to be registered with the system so that standard
-    rewriting tactics work for them almost as well as for equalities.)
-    But it is worth knowing about, because it applies even in
-    situations where the equivalence in question is _not_ over
-    functions.  For example, if we chose to represent state mappings
-    as binary search trees, we would need to use an explicit
-    equivalence of this kind. *)
-(** 概して、この明示的な同値のアプローチは、関数外延性を使うものよりかなり難しくなります。
-    (Coqは"setoids"という先進的な仕組みを持っています。
-    setoid は同値関係の扱いをいくらか容易にします。
-    その方法は、同値関係をシステムに登録すると、
-    それを使った書き換えタクティックが、もとの等しさ(equality)
-    に対してとほとんど同じようにはたらくようになるというものです。)
-    しかしこの、状態の同値を明示的に記述する方法は知っておく価値があります。
-    なぜなら、この方法は、問題となる同値が関数についてのもの「ではない」状況でも使えるからです。
-    例えば、状態の写像を二分探索木を使って行ったとすると、
-    このような明示的な同値を使う必要があるでしょう。*)
-
-(* ####################################################### *)
 (* * Additional Exercises *)
 (** * さらなる練習問題 *)
 
-(* **** Exercise: 4 stars, optional (for_while_equiv) *)
 (** **** 練習問題: ★★★★, optional (for_while_equiv) *)
-(* This exercise extends the optional add_for_loop exercise from
-    Imp.v, where you were asked to extend the language of commands
-    with C-style [for] loops.  Prove that the command:
+(* This exercise extends the optional [add_for_loop] exercise from
+    the [Imp] chapter, where you were asked to extend the language 
+    of commands with C-style [for] loops.  Prove that the command:
+
       for (c1 ; b ; c2) {
           c3
       }
+
     is equivalent to:
-       c1 ; 
+
+       c1 ;
        WHILE b DO
          c3 ;
          c2
@@ -2260,7 +2073,7 @@ Proof.
 (** この練習問題は、Imp_J.vのoptionalの練習問題 add_for_loop を拡張したものです。
     もとの add_for_loop は、コマンド言語に C-言語のスタイルの [for]ループを
     拡張しなさい、というものでした。
-    ここでは次のことを証明しなさい:    
+    ここでは次のことを証明しなさい:   
       for (c1 ; b ; c2) {
           c3
       }
@@ -2275,18 +2088,68 @@ Proof.
 (* FILL IN HERE *)
 (** [] *)
 
-(* **** Exercise: 3 stars, optional (swap_noninterfering_assignments) *)
 (** **** 練習問題: ★★★, optional (swap_noninterfering_assignments) *)
+(*  (Hint: You'll need [functional_extensionality] for this one.) *)
+(** (ヒント: [functional_extensionality]が必要になるでしょう。*)
+
 Theorem swap_noninterfering_assignments: forall l1 l2 a1 a2,
-  l1 <> l2 -> 
+  l1 <> l2 ->
   var_not_used_in_aexp l1 a2 ->
   var_not_used_in_aexp l2 a1 ->
   cequiv
     (l1 ::= a1;; l2 ::= a2)
     (l2 ::= a2;; l1 ::= a1).
-Proof. 
-(* Hint: You'll need [functional_extensionality] *)
-(* ヒント: [functional_extensionality]を必要とするでしょう。 *)
+Proof.
 (* FILL IN HERE *) Admitted.
 (** [] *)
+
+(** **** 練習問題: ★★★★, advanced, optional (capprox) *)
+
+(** In this exercise we define an asymmetric variant of program
+    equivalence we call _program approximation_. We say that a
+    program [c1] _approximates_ a program [c2] when, for each of
+    the initial states for which [c1] terminates, [c2] also terminates
+    and produces the same final state. Formally, program approximation
+    is defined as follows: *)
+(** この練習問題では、プログラムの同値性の正反対の変奏を定義します。*)
+
+Definition capprox (c1 c2 : com) : Prop := forall (st st' : state),
+  c1 / st \\ st' -> c2 / st \\ st'.
+
+(** For example, the program [c1 = WHILE X <> 1 DO X ::= X - 1 END]
+    approximates [c2 = X ::= 1], but [c2] does not approximate [c1]
+    since [c1] does not terminate when [X = 0] but [c2] does.  If two
+    programs approximate each other in both directions, then they are
+    equivalent. *)
+
+(** Find two programs [c3] and [c4] such that neither approximates
+    the other. *)
+
+Definition c3 : com := (* FILL IN HERE *) admit.
+Definition c4 : com := (* FILL IN HERE *) admit.
+
+Theorem c3_c4_different : ~ capprox c3 c4 /\ ~ capprox c4 c3.
+Proof. (* FILL IN HERE *) Admitted.
+
+(** Find a program [cmin] that approximates every other program. *)
+
+Definition cmin : com :=
+  (* FILL IN HERE *) admit.
+
+Theorem cmin_minimal : forall c, capprox cmin c.
+Proof. (* FILL IN HERE *) Admitted.
+
+(** Finally, find a non-trivial property which is preserved by
+    program approximation (when going from left to right). *)
+
+Definition zprop (c : com) : Prop :=
+  (* FILL IN HERE *) admit.
+
+
+Theorem zprop_preserving : forall c c',
+  zprop c -> capprox c c' -> zprop c'.
+Proof. (* FILL IN HERE *) Admitted.
+(** [] *)
+
+(** $Date: 2016-05-26 16:17:19 -0400 (Thu, 26 May 2016) $ *)
 
